Fir/Wasm/Concrete.lean
@@ -13,6 +13,7 @@ import Fir.Wasm.Concrete.ClosureProjectionCorrectness
 import Fir.Wasm.Concrete.ObjectFieldsCorrectness
 import Fir.Wasm.Concrete.FreshAllocationCorrectness
 import Fir.Wasm.Concrete.HeapRefinement
+import Fir.Wasm.Concrete.ArrayAllocationCorrectness
 import Fir.Wasm.Concrete.NaturalAllocationCorrectness
 import Fir.Wasm.Concrete.IntegerAllocationCorrectness
 import Fir.Wasm.Concrete.PromotedTagCorrectness
